src/OpaqueOps.v
@@ -2,34 +2,235 @@ Require Import Common.
 Require Import HList.
 Require Import SafeInt.
 Require Import Utopia.
+Require Import Monads.
+
 Require Import OpaqueTypes.
+
 Require Import SourceValues.
+Require HighestValues.
+
+Require Import MatchValues.
+
+Local Open Scope option_monad.
+
+
+Inductive opaque_oper_name : Set :=
+| ONadd
+| ONtest.
 
 Inductive opaque_oper : list type -> type -> Set :=
 | Oadd : opaque_oper [Opaque Oint; Opaque Oint] (Opaque Oint)
 | Otest : opaque_oper [Opaque Oint] (ADT Tbool)
 .
 
-
-Definition opaque_oper_denote {atys rty} (op : opaque_oper atys rty) :
-        hlist type_denote atys -> type_denote rty :=
+Definition opaque_oper_to_name {atys rty} (op : opaque_oper atys rty) : opaque_oper_name :=
     match op with
-    | Oadd => fun args => Int.add (hhead args) (hhead (htail args))
-    | Otest => fun args => Int.eq (hhead args) Int.zero
+    | Oadd => ONadd
+    | Otest => ONtest
     end.
+
+
 
 Definition unwrap_opaque {G oty} (v : value G (Opaque oty)) : opaque_type_denote oty :=
     match v in value _ (Opaque oty_) return opaque_type_denote oty_ with
     | VOpaque v => v
     end.
 
+
+Fixpoint hmap_map {A A'} {B : A' -> Type} (f : A -> A') {xs : list A}
+        (h : hlist B (map f xs)) : hlist (fun x => B (f x)) xs :=
+    match xs as xs_ return hlist B (map f xs_) -> hlist _ xs_ with
+    | [] => fun _ => hnil
+    | x :: xs =>
+            case_hlist_cons _ (fun (y : B (f x)) ys =>
+                let ys' := hmap_map f ys in
+                hcons y ys'
+            ) 
+    end h.
+
+Definition type_denote_map_opaque {otys} :
+        hlist type_denote (map Opaque otys) ->
+        hlist opaque_type_denote otys :=
+    hmap_map Opaque.
+
+Definition unwrap_opaque_hlist {G otys} (vs : hlist (value G) (map Opaque otys)) :
+        hlist opaque_type_denote otys.
+induction otys.
+  { constructor. }
+invc vs. constructor; eauto using unwrap_opaque.
+Defined.
+
+Lemma unwrap_opaque_hlist_is_hmap :
+    forall G otys (vs : hlist (value G) (map Opaque otys)),
+    unwrap_opaque_hlist vs = hmap (fun _ v => unwrap_opaque v) (hmap_map Opaque vs).
+induction otys; intros.
+- reflexivity.
+- pattern vs. simple refine (case_hlist_cons _ _ vs).
+  intros. simpl.
+  rewrite <- IHotys. reflexivity.
+Qed.
+
+Definition unwrap_highest oty (v : HighestValues.value) :
+        option (opaque_type_denote oty).
+refine (
+    match v with
+    | HighestValues.Opaque vty v =>
+        if opaque_type_name_eq_dec oty vty then Some _ else None
+    | _ => None
+    end
+).
+rewrite e. exact v.
+Defined.
+
+Definition unwrap_highest_hlist otys (vs : list HighestValues.value) :
+        option (hlist opaque_type_denote otys) :=
+    let fix go otys vs :=
+        match otys as otys_ return option (hlist _ otys_) with
+        | [] => Some hnil
+        | oty :: otys =>
+                match vs with
+                | [] => None
+                | v :: vs =>
+                        unwrap_highest oty v >>= fun v' =>
+                        go otys vs >>= fun vs' =>
+                        Some (hcons v' vs')
+                end
+        end in
+    go otys vs.
+
+
+
+Definition oper_implH atys rty :=
+    hlist opaque_type_denote atys ->
+    opaque_type_denote rty.
+
+Definition liftH {atys rty} (f : oper_implH atys rty) :
+        hlist type_denote (map Opaque atys) -> type_denote (Opaque rty) :=
+    fun args => f (type_denote_map_opaque args).
+
+Definition liftH_source {G atys rty} (f : oper_implH atys rty) :
+        hlist (value G) (map Opaque atys) -> value G (Opaque rty) :=
+    fun args => VOpaque (f (unwrap_opaque_hlist args)).
+
+Definition liftH_highest {atys rty} (f : oper_implH atys rty) :
+        list HighestValues.value -> option HighestValues.value :=
+    fun args =>
+        unwrap_highest_hlist atys args >>= fun args' =>
+        Some (HighestValues.Opaque rty (f args')).
+
+
+
+
+Lemma value_denote_unwrap_opaque :
+    forall G (h : hlist func_type_denote G) oty (v : value G (Opaque oty)),
+    value_denote h v = unwrap_opaque v.
+intros.
+pattern v.
+refine match v as v_ in value _ (Opaque oty_) return _ v_ with
+| VOpaque v => _
+end.
+reflexivity.
+Qed.
+
+Lemma type_denote_map_opaque_unwrap_opaque_hlist :
+    forall G (h : hlist func_type_denote G)
+        otys (vs : hlist (value G) (map Opaque otys)),
+    type_denote_map_opaque (hmap (@value_denote G h) vs) =
+    unwrap_opaque_hlist vs.
+intros. rewrite unwrap_opaque_hlist_is_hmap.
+unfold type_denote_map_opaque.
+induction otys.
+- simpl. reflexivity.
+- pattern vs. simple refine (case_hlist_cons _ _ vs).
+  intros. simpl.
+  rewrite <- IHotys. rewrite value_denote_unwrap_opaque. reflexivity.
+Qed.
+
+Lemma liftH_source_sim :
+    forall G (h : hlist func_type_denote G) atys rty (f : oper_implH atys rty)
+        (vs : hlist (value G) (map Opaque atys)),
+    liftH f (hmap (@value_denote G h) vs) =
+    value_denote h (liftH_source f vs).
+intros. simpl. unfold liftH.
+revert f vs. induction atys; intros.
+- reflexivity.
+- f_equal. apply type_denote_map_opaque_unwrap_opaque_hlist.
+Qed.
+
+
+Lemma compile_highest_unwrap :
+    forall G oty (v : value G (Opaque oty)),
+    Some (unwrap_opaque v) = unwrap_highest oty (MatchValues.compile_highest v).
+intros.
+pattern oty, v.
+refine match v as v_ in value _ (Opaque oty_) return _ oty_ v_ with
+| VOpaque v => _
+end.
+simpl. break_match; try congruence. f_equal.
+unfold eq_rect_r. fix_eq_rect. reflexivity.
+Qed.
+
+Lemma compile_highest_unwrap_hlist :
+    forall G otys (vs : hlist (value G) (map Opaque otys)),
+    Some (unwrap_opaque_hlist vs) =
+    unwrap_highest_hlist otys (MatchValues.compile_highest_list vs).
+induction otys; intros.
+- reflexivity.
+- pattern vs. simple refine (case_hlist_cons _ _ vs).
+  intros. simpl.
+  rewrite <- IHotys.
+  rewrite <- compile_highest_unwrap.
+  reflexivity.
+Qed.
+
+Lemma liftH_highest_sim :
+    forall G (h : hlist func_type_denote G) atys rty (f : oper_implH atys rty)
+        (vs : hlist (value G) (map Opaque atys)),
+    Some (MatchValues.compile_highest (liftH_source f vs)) =
+    liftH_highest f (MatchValues.compile_highest_list vs).
+intros. simpl. unfold liftH_highest. 
+induction atys; intros.
+- reflexivity.
+- rewrite <- compile_highest_unwrap_hlist. cbn [bind_option].
+  reflexivity.
+Qed.
+
+
+
+Definition oper_impl2 aty1 aty2 rty :=
+    opaque_type_denote aty1 ->
+    opaque_type_denote aty2 ->
+    opaque_type_denote rty.
+
+Definition lift2H {aty1 aty2 rty} :
+        oper_impl2 aty1 aty2 rty -> oper_implH [aty1; aty2] rty :=
+    fun f => fun args => f (hhead args) (hhead (htail args)).
+
+Definition lift2 {aty1 aty2 rty} (f : oper_impl2 aty1 aty2 rty) :
+        hlist type_denote (map Opaque [aty1; aty2]) -> type_denote (Opaque rty) :=
+    liftH (lift2H f).
+
+Definition lift2_source {G aty1 aty2 rty} (f : oper_impl2 aty1 aty2 rty) :
+        hlist (value G) (map Opaque [aty1; aty2]) -> value G (Opaque rty) :=
+    liftH_source (lift2H f).
+
+Definition lift2_highest {aty1 aty2 rty} (f : oper_impl2 aty1 aty2 rty) :
+        list HighestValues.value -> option HighestValues.value :=
+    liftH_highest (lift2H f).
+
+
+
+Definition opaque_oper_denote {atys rty} (op : opaque_oper atys rty) :
+        hlist type_denote atys -> type_denote rty :=
+    match op with
+    | Oadd => @lift2 Oint Oint Oint  Int.add
+    | Otest => fun args => Int.eq (hhead args) Int.zero
+    end.
+
 Definition opaque_oper_denote_source {G atys rty} (op : opaque_oper atys rty) :
         hlist (value G) atys -> value G rty :=
     match op with
-    | Oadd => fun args =>
-            let x := unwrap_opaque (hhead args) in
-            let y := unwrap_opaque (hhead (htail args)) in
-            VOpaque (oty := Oint) (Int.add x y)
+    | Oadd => @lift2_source _ Oint Oint Oint  Int.add
     | Otest => fun args =>
             let x := unwrap_opaque (hhead args) in
             if Int.eq x Int.zero then
@@ -37,3 +238,41 @@ Definition opaque_oper_denote_source {G atys rty} (op : opaque_oper atys rty) :
             else
                 VConstr CTfalse hnil
     end.
+
+Definition opaque_oper_denote_highest (op : opaque_oper_name) :
+        list HighestValues.value -> option HighestValues.value :=
+    match op with
+    | ONadd => @lift2_highest Oint Oint Oint  Int.add
+    | ONtest => fun args =>
+        unwrap_highest_hlist [Oint] args >>= fun args' =>
+        if Int.eq (hhead args') Int.zero
+           then Some (HighestValues.Constr Ctrue [])
+           else Some (HighestValues.Constr Cfalse [])
+    end.
+
+
+Lemma opaque_oper_source_sim :
+    forall G (h : hlist func_type_denote G) atys rty (op : opaque_oper atys rty)
+        (vs : hlist (value G) atys),
+    opaque_oper_denote op (hmap (@value_denote G h) vs) =
+    value_denote h (opaque_oper_denote_source op vs).
+destruct op; intros; try solve [eapply liftH_source_sim]; simpl.
+- (* Otest *)
+  pattern vs. simple refine (case_hlist_cons _ _ vs).  intros. simpl.
+  rewrite value_denote_unwrap_opaque.
+  break_match. all: reflexivity.
+Qed.
+
+Lemma opaque_oper_highest_sim :
+    forall G (h : hlist func_type_denote G) atys rty (op : opaque_oper atys rty)
+        (vs : hlist (value G) atys),
+    Some (MatchValues.compile_highest (opaque_oper_denote_source op vs)) =
+    opaque_oper_denote_highest (opaque_oper_to_name op)
+        (MatchValues.compile_highest_list vs).
+destruct op; intros; try solve [eapply liftH_highest_sim; eauto]; simpl.
+- (* Otest *)
+  pattern vs. simple refine (case_hlist_cons _ _ vs).  intros. simpl.
+  rewrite <- compile_highest_unwrap. simpl.
+  break_match; simpl; reflexivity.
+Qed.
+
